Use blocks to identify entry point in language interfaces
There are aspects to this change.

First, at the assemby level we will no longer have function identifiers
in queries, but simply the current value of the program counter.
Relating this to the C language interface would require the global
environments to be involved if we have function names in C-level
queries. If instead we use the block from the beginning to identify the
function being called, there is no problem.

Second, there is a discrepancy between the way Compcert names internal
functions (using AST.ident), and external function (using string).
Before, as asssumed there was some mapping str2ident and used that to
fill the gap. Now, we identify external function by their declaration in
the program (so, the corresponding block, although this could have been
the corresponding AST.ident in the old interface as well).

backend/CminorSel.v
@@ -448,22 +448,21 @@ Inductive step: state -> trace -> state -> Prop :=
 
 End RELSEM.
 
-Inductive initial_state (p: program): query li_c -> state -> Prop :=
-  | initial_state_intro: forall id b f vargs m,
-      let ge := Genv.globalenv p in
+Inductive initial_state (ge: genv): query li_c -> state -> Prop :=
+  | initial_state_intro: forall b f vargs m,
       Ple (Genv.genv_next ge) (Mem.nextblock m) ->
-      Genv.find_symbol ge (str2ident id) = Some b ->
       Genv.find_funct_ptr ge b = Some (Internal f) ->
       Val.has_type_list vargs (sig_args (fn_sig f)) ->
-      initial_state p
-        (cq id (fn_sig f) vargs m)
+      initial_state ge
+        (cq b (fn_sig f) vargs m)
         (Callstate (Internal f) vargs Kstop m).
 
-Inductive at_external: state -> query li_c -> Prop :=
-  | at_external_intro id sg vargs k m:
-      at_external
+Inductive at_external (ge: genv): state -> query li_c -> Prop :=
+  | at_external_intro b id sg vargs k m:
+      Genv.find_funct_ptr ge b = Some (External (EF_external id sg)) ->
+      at_external ge
         (Callstate (External (EF_external id sg)) vargs k m)
-        (cq id sg vargs m).
+        (cq b sg vargs m).
 
 Inductive after_external: state -> reply li_c -> state -> Prop :=
   | after_external_intro id sg vargs k m vres m':
@@ -477,13 +476,14 @@ Inductive final_state: state -> reply li_c -> Prop :=
       final_state (Returnstate r Kstop m) (r, m).
 
 Definition semantics (p: program) :=
+  let ge := Genv.globalenv p in
   Semantics li_c li_c
     step
-    (initial_state p)
-    at_external
+    (initial_state ge)
+    (at_external ge)
     after_external
     final_state
-    (Genv.globalenv p).
+    ge.
 
 Hint Constructors eval_expr eval_exprlist eval_condexpr: evalexpr.
 
