backend/Linear.v
@@ -253,22 +253,21 @@ Inductive step: state -> trace -> state -> Prop :=
 
 End RELSEM.
 
-Inductive initial_state (p: program): query li_locset -> state -> Prop :=
-  | initial_state_intro: forall id b f rs m,
-      let ge := Genv.globalenv p in
+Inductive initial_state (ge: genv): query li_locset -> state -> Prop :=
+  | initial_state_intro: forall b f rs m,
       Ple (Genv.genv_next ge) (Mem.nextblock m) ->
-      Genv.find_symbol ge (str2ident id) = Some b ->
       Genv.find_funct_ptr ge b = Some f ->
       (forall l, Val.has_type (rs l) (Loc.type l)) ->
-      initial_state p
-        (lq id (funsig f) rs m)
+      initial_state ge
+        (lq b (funsig f) rs m)
         (Callstate (Parent rs :: nil) f rs m).
 
-Inductive at_external: state -> query li_c -> Prop :=
-  | at_external_intro id sg s rs m:
-      at_external
+Inductive at_external (ge: genv): state -> query li_c -> Prop :=
+  | at_external_intro b id sg s rs m:
+      Genv.find_funct_ptr ge b = Some (External (EF_external id sg)) ->
+      at_external ge
         (Callstate s (External (EF_external id sg)) rs m)
-        (cq id sg (map (fun p => Locmap.getpair p rs) (loc_arguments sg)) m).
+        (cq b sg (map (fun p => Locmap.getpair p rs) (loc_arguments sg)) m).
 
 Inductive after_external: state -> reply li_c -> state -> Prop :=
   | after_external_intro id sg s rs m vres m':
@@ -282,10 +281,11 @@ Inductive final_state: state -> reply li_locset -> Prop :=
       final_state (Returnstate (Parent init_rs :: s) rs m) (rs, m).
 
 Definition semantics (p: program) :=
+  let ge := Genv.globalenv p in
   Semantics li_c li_locset
     step
-    (initial_state p)
-    at_external
+    (initial_state ge)
+    (at_external ge)
     after_external
     final_state
-    (Genv.globalenv p).
+    ge.
